theories/URI.v
@@ -1,10 +1,15 @@
+From Coq Require Import List.
 From Praecia Require Import Parser.
-From Prelude Require Import Option.
+From Prelude Require Import Option Equality.
+
+Import ListNotations.
+#[local] Open Scope string_scope.
+#[local] Open Scope prelude_scope.
 
 Fixpoint of_ascii_list (l : list ascii) : string :=
   match l with
-  | cons x rst => String x (of_ascii_list rst)
-  | nil => EmptyString
+  | x :: rst => String x (of_ascii_list rst)
+  | [] => EmptyString
   end.
 
 Inductive directory_id : Type :=
@@ -17,33 +22,48 @@ Inductive uri := make_uri { dirname : list directory_id
                           }.
 
 #[local]
-Fixpoint canonicalize_aux (acc : list directory_id) (dirids : list directory_id) : list directory_id :=
+Fixpoint canonicalize_aux (acc : list directory_id) (dirids : list directory_id)
+  : list directory_id :=
   match dirids with
-  | cons Current rst => canonicalize_aux acc rst
-  | cons Parent rst => canonicalize_aux (List.tl acc) rst
-  | cons x rst => canonicalize_aux (cons x acc) rst
-  | nil => List.rev acc
+  | Current :: rst => canonicalize_aux acc rst
+  | Parent :: rst => canonicalize_aux (tl acc) rst
+  | x :: rst => canonicalize_aux (x :: acc) rst
+  | [] => rev acc
   end.
 
-Definition canonicalize := canonicalize_aux nil.
+Definition canonicalize := canonicalize_aux [].
 
 Definition dirname_eq (d1 d2: list directory_id) : Prop :=
   canonicalize d1 = canonicalize d2.
 
 Inductive canonical : list directory_id -> Prop :=
-| canonical_nil : canonical nil
-| canonical_cons (s : string) (rst : list directory_id) (canonical_rst : canonical rst)
-  : canonical (cons (Dirname s) rst).
+| canonical_nil : canonical []
+| canonical_cons
+    (s : string) (rst : list directory_id) (canonical_rst : canonical rst)
+  : canonical (Dirname s :: rst).
+
+Lemma canonical_canonical_tl (d : list directory_id)
+  : canonical d -> canonical (tl d).
+
+Proof.
+Admitted.
+
+Lemma canonical_canonical_rev (d : list directory_id)
+  : canonical d <-> canonical (rev d).
+
+Proof.
+Admitted.
 
 #[local]
-Lemma canonicalize_aux_canonical (d acc : list directory_id) (acc_canon : canonical acc)
+Lemma canonicalize_aux_canonical (d acc : list directory_id)
+    (acc_canon : canonical acc)
   : canonical (canonicalize_aux acc d).
 
 Proof.
   revert acc acc_canon.
   induction d; intros acc acc_canon.
   + cbn.
-    admit.
+    now rewrite <- canonical_canonical_rev.
   + destruct a.
     ++ cbn.
        apply IHd.
@@ -52,8 +72,8 @@ Proof.
        now apply IHd.
     ++ cbn.
        apply IHd.
-       admit.
-Admitted.
+       now apply canonical_canonical_tl.
+Qed.
 
 Lemma canonicalize_canonical (d : list directory_id)
   : canonical (canonicalize d).
@@ -63,10 +83,16 @@ Proof.
   constructor.
 Qed.
 
-Remark canonical_canonicalize_cons_equ (s : string) (d : list directory_id) (canon : canonical d)
-  : canonicalize (cons (Dirname s) d) = cons (Dirname s) (canonicalize d).
+Remark canonical_canonicalize_cons_equ (s : string)
+    (d : list directory_id) (canon : canonical d)
+  : canonicalize (Dirname s :: d) = Dirname s :: canonicalize d.
 
 Proof.
+  induction d.
+  + reflexivity.
+  + inversion canon; subst.
+    rename s0 into s'.
+    cbn.
 Admitted.
 
 Lemma canonicalize_canonical_equ (d : list directory_id) (canon : canonical d)
@@ -88,15 +114,13 @@ Proof.
   apply canonicalize_canonical.
 Qed.
 
-Search (string -> string -> string).
-
 #[program, local]
 Fixpoint uri_to_path_aux (d : list directory_id) (canon : canonical d) : string :=
   match d with
-  | nil => EmptyString
-  | cons (Dirname x) rst => append x (append "/" (uri_to_path_aux rst _))
-  | cons Parent _ => _
-  | cons Current _ => _
+  | [] => EmptyString
+  | Dirname x :: rst => x ++ "/" ++ uri_to_path_aux rst _
+  | Parent :: _ => _
+  | Current :: _ => _
   end.
 
 Next Obligation.
@@ -111,11 +135,9 @@ Next Obligation.
   exfalso; inversion canon.
 Defined.
 
-Search (?a -> option ?a -> ?a).
-
 #[program]
 Definition uri_to_path (u : uri) : string :=
-  append (uri_to_path_aux (canonicalize (dirname u)) _) (fromMaybe ""%string (filename u)).
+  uri_to_path_aux (canonicalize (dirname u)) _ ++ fromMaybe ""%string (filename u).
 
 Next Obligation.
   apply canonicalize_canonical.
@@ -123,7 +145,8 @@ Qed.
 
 (** * Parsing URI *)
 
-Definition dir_id_sep := peak (eoi <|> ((char " " <|> char "/") *> pure tt)).
+Definition dir_id_sep : parser unit :=
+  peak (eoi <|> ((char " " <|> char "/") *> pure tt)).
 
 Definition dirid : parser directory_id :=
   many (char "/") *>
@@ -134,7 +157,7 @@ Definition dirid : parser directory_id :=
           pure (Dirname (of_ascii_list name))
        end).
 
-(* TODO: bad performance, can we provide some useful hints here? *)
+(* TODO: poor performance, can we provide some useful hints here? *)
 Definition path_dirname : parser (list directory_id) :=
   many dirid.
 
@@ -142,7 +165,7 @@ Definition read_uri : parser uri :=
   do var dirname <- path_dirname in
      many (char "/");
      var maybe_filename <- many_until read_char (char " ") in
-     pure (make_uri dirname (if Nat.eqb (List.length maybe_filename) 0
+     pure (make_uri dirname (if List.length maybe_filename =? 0
                              then None
                              else Some (of_ascii_list maybe_filename)))
   end.
