theories/HTTP.v
@@ -1,6 +1,10 @@
 From FreeSpec Require Import Core.
 From Praecia Require Import Parser URI FileSystem TCP.
 
+Import ListNotations.
+#[local] Open Scope string_scope.
+#[local] Open Scope prelude_scope.
+
 Generalizable All Variables.
 
 Inductive request :=
@@ -11,11 +15,25 @@ Inductive status :=
 | client_error_BadRequest
 | client_error_NotFound.
 
+Definition status_to_string (code : status) : string :=
+  match code with
+  | success_OK => "200"
+  | client_error_BadRequest => "400"
+  | client_error_NotFound => "404"
+  end.
+
 Record response := make_response { code : status
                                  ; body : string
                                  }.
 
-Axiom response_to_string : response -> string.
+#[local] Open Scope string_scope.
+
+Definition newline := String "010" "".
+
+Definition response_to_string (res : response) : string :=
+  "HTTP/1.1 " ++ status_to_string (code res) ++ " Reason phrase" ++ newline ++
+  newline ++
+  body res.
 
 Definition http_request : parser request :=
   Get <$> (str "GET" *> whitespaces *> read_uri <* whitespaces <* str "HTTP/1.1").
